lib/smack/Translator.cpp
@@ -31,10 +31,17 @@ namespace smack{
         std::list<const SpatialLiteral*> spatialList = shExpr->getSpatialExpr();
         CDEBUG(std::cout << "======center test: in spatial translate process======\n");
         z3::expr_vector z3SpatialAtoms(*z3Ctx);
+        bool hasSpatials = false;
         for(const SpatialLiteral* sp : spatialList){
-            z3SpatialAtoms.push_back(
-                sp->translateToZ3(*z3Ctx, cfg, varFac)
-            );
+            if(hasSpatials && SpatialLiteral::Kind::EMP == sp->getId()){
+                continue;
+            }
+            z3::expr z3sp = sp->translateToZ3(*z3Ctx, cfg, varFac);
+            z3SpatialAtoms.push_back(z3sp);
+            hasSpatials = true;
+        }
+        if(!hasSpatials){
+            z3SpatialAtoms.push_back(slah_api::newEmp(*z3Ctx));
         }
         z3::expr exp = slah_api::newSep(z3SpatialAtoms);
         CDEBUG(std::cout << exp.to_string() << std::endl; )
