testcases/printtest/exec.c
@@ -14,25 +14,45 @@ typedef struct {
 
 
 int main(){
-    int num = 5;
-    int *j = (int*)malloc(num*sizeof(int));
-    int nnum = *(j+1) + (-1); 
-    free(j);
+    // int num = 5;
+    // int *j = (int*)malloc(num*sizeof(int));
+    // int nnum = *(j+1) + (-1); 
+    // free(j);
 
-// // new example
-//     TData data;
-//     TData* pdata = &data;
-//     pdata->lo = malloc(16);
-//     pdata->hi = malloc(24);
-//     void *lo = pdata->lo;
-//     void *hi = pdata->hi;
+// new example
+    // TData data;
+    // TData* pdata = &data;
 
-//     if (lo == hi) {
-//         free(lo);
-//         free(hi);
-//     }
+    // TData a = *(pdata-1);
+    // int b = (int)a.lo;
 
-//     pdata->lo = (void *) 0;
-//     pdata->hi = (void *) 0;
-    
-}
+    // TData c;
+    // c.lo = 0;
+    // pdata->lo = malloc(16);
+    // pdata->hi = malloc(24);
+    // void *lo = pdata->lo;
+    // void *hi = pdata->hi;
+
+    // if (lo == hi) {
+    //     free(lo);
+    //     free(hi);
+    // }
+
+    // pdata->lo = (void *) 0;
+    // pdata->hi = (void *) 0;
+
+    // test_type i;
+    // i.a = 0;
+    // i.b = 100;
+    // int a = i.b;
+    // i.next = malloc(sizeof(test_type));
+    // i.next->a = 1;
+    // i.next->b = 101;
+
+    int a[10];
+    int num = 101;
+    int b[num+1];
+    a[2] = 111;
+    b[3] = 222;
+    int newname = a[1];
+} 
