testcases/printtest/exec_IR.ll
@@ -1,33 +1,38 @@
-; ModuleID = '/home/clexma/Desktop/Disk_D/Tools/SMACK/smack/build/b-wwnyj34i.bc'
+; ModuleID = '/home/clexma/Desktop/Disk_D/Tools/SMACK/smack/build/b-jvwhf68y.bc'
 source_filename = "llvm-link"
 target datalayout = "e-m:e-p270:32:32-p271:32:32-p272:64:64-i64:64-f80:128-n8:16:32:64-S128"
 target triple = "x86_64-pc-linux-gnu"
 
 ; Function Attrs: noinline nounwind uwtable
-define dso_local i32 @main() #0 !dbg !10 {
-  call void @llvm.dbg.value(metadata i32 5, metadata !13, metadata !DIExpression()), !dbg !14, !verifier.code !15
-  %1 = sext i32 5 to i64, !dbg !16, !verifier.code !15
-  %2 = mul i64 %1, 4, !dbg !17, !verifier.code !15
-  %3 = call noalias i8* @malloc(i64 %2) #3, !dbg !18, !verifier.code !15
-  %4 = bitcast i8* %3 to i32*, !dbg !19, !verifier.code !15
-  call void @llvm.dbg.value(metadata i32* %4, metadata !20, metadata !DIExpression()), !dbg !14, !verifier.code !15
-  %5 = getelementptr inbounds i32, i32* %4, i64 1, !dbg !21, !verifier.code !15
-  %6 = load i32, i32* %5, align 4, !dbg !22, !verifier.code !15
-  %7 = add nsw i32 %6, -1, !dbg !23, !verifier.code !15
-  call void @llvm.dbg.value(metadata i32 %7, metadata !24, metadata !DIExpression()), !dbg !14, !verifier.code !15
-  %8 = bitcast i32* %4 to i8*, !dbg !25, !verifier.code !15
-  call void @free(i8* %8) #3, !dbg !26, !verifier.code !15
-  ret i32 0, !dbg !27, !verifier.code !15
+define dso_local i32 @main() #0 !dbg !7 {
+  %1 = alloca [10 x i32], align 16, !verifier.code !11
+  call void @llvm.dbg.declare(metadata [10 x i32]* %1, metadata !12, metadata !DIExpression()), !dbg !16, !verifier.code !11
+  call void @llvm.dbg.value(metadata i32 101, metadata !17, metadata !DIExpression()), !dbg !18, !verifier.code !11
+  %2 = add nsw i32 101, 1, !dbg !19, !verifier.code !11
+  %3 = zext i32 %2 to i64, !dbg !20, !verifier.code !11
+  %4 = call i8* @llvm.stacksave(), !dbg !20, !verifier.code !11
+  %5 = alloca i32, i64 %3, align 16, !dbg !20, !verifier.code !11
+  call void @llvm.dbg.value(metadata i64 %3, metadata !21, metadata !DIExpression()), !dbg !18, !verifier.code !11
+  call void @llvm.dbg.declare(metadata i32* %5, metadata !23, metadata !DIExpression()), !dbg !27, !verifier.code !11
+  %6 = getelementptr inbounds [10 x i32], [10 x i32]* %1, i64 0, i64 2, !dbg !28, !verifier.code !11
+  store i32 111, i32* %6, align 8, !dbg !29, !verifier.code !11
+  %7 = getelementptr inbounds i32, i32* %5, i64 3, !dbg !30, !verifier.code !11
+  store i32 222, i32* %7, align 4, !dbg !31, !verifier.code !11
+  %8 = getelementptr inbounds [10 x i32], [10 x i32]* %1, i64 0, i64 1, !dbg !32, !verifier.code !11
+  %9 = load i32, i32* %8, align 4, !dbg !32, !verifier.code !11
+  call void @llvm.dbg.value(metadata i32 %9, metadata !33, metadata !DIExpression()), !dbg !18, !verifier.code !11
+  call void @llvm.stackrestore(i8* %4), !dbg !34, !verifier.code !11
+  ret i32 0, !dbg !34, !verifier.code !11
 }
 
 ; Function Attrs: nounwind readnone speculatable willreturn
 declare void @llvm.dbg.declare(metadata, metadata, metadata) #1
 
 ; Function Attrs: nounwind
-declare dso_local noalias i8* @malloc(i64) #2
+declare i8* @llvm.stacksave() #2
 
 ; Function Attrs: nounwind
-declare dso_local void @free(i8*) #2
+declare void @llvm.stackrestore(i8*) #2
 
 ; Function Attrs: nounwind readnone speculatable willreturn
 declare void @llvm.dbg.value(metadata, metadata, metadata) #1
@@ -39,38 +44,44 @@ entry:
 
 attributes #0 = { noinline nounwind uwtable "correctly-rounded-divide-sqrt-fp-math"="false" "disable-tail-calls"="false" "frame-pointer"="all" "less-precise-fpmad"="false" "min-legal-vector-width"="0" "no-infs-fp-math"="false" "no-jump-tables"="false" "no-nans-fp-math"="false" "no-signed-zeros-fp-math"="false" "no-trapping-math"="false" "stack-protector-buffer-size"="8" "target-cpu"="x86-64" "target-features"="+cx8,+fxsr,+mmx,+sse,+sse2,+x87" "unsafe-fp-math"="false" "use-soft-float"="false" }
 attributes #1 = { nounwind readnone speculatable willreturn }
-attributes #2 = { nounwind "correctly-rounded-divide-sqrt-fp-math"="false" "disable-tail-calls"="false" "frame-pointer"="all" "less-precise-fpmad"="false" "no-infs-fp-math"="false" "no-nans-fp-math"="false" "no-signed-zeros-fp-math"="false" "no-trapping-math"="false" "stack-protector-buffer-size"="8" "target-cpu"="x86-64" "target-features"="+cx8,+fxsr,+mmx,+sse,+sse2,+x87" "unsafe-fp-math"="false" "use-soft-float"="false" }
-attributes #3 = { nounwind }
+attributes #2 = { nounwind }
 
 !llvm.dbg.cu = !{!0}
-!llvm.ident = !{!6}
-!llvm.module.flags = !{!7, !8, !9}
+!llvm.ident = !{!3}
+!llvm.module.flags = !{!4, !5, !6}
 
-!0 = distinct !DICompileUnit(language: DW_LANG_C99, file: !1, producer: "clang version 10.0.0-4ubuntu1 ", isOptimized: false, runtimeVersion: 0, emissionKind: FullDebug, enums: !2, retainedTypes: !3, splitDebugInlining: false, nameTableKind: None)
+!0 = distinct !DICompileUnit(language: DW_LANG_C99, file: !1, producer: "clang version 10.0.0-4ubuntu1 ", isOptimized: false, runtimeVersion: 0, emissionKind: FullDebug, enums: !2, splitDebugInlining: false, nameTableKind: None)
 !1 = !DIFile(filename: "../testcases/printtest/exec.c", directory: "/home/clexma/Desktop/Disk_D/Tools/SMACK/smack/build")
 !2 = !{}
-!3 = !{!4}
-!4 = !DIDerivedType(tag: DW_TAG_pointer_type, baseType: !5, size: 64)
-!5 = !DIBasicType(name: "int", size: 32, encoding: DW_ATE_signed)
-!6 = !{!"clang version 10.0.0-4ubuntu1 "}
-!7 = !{i32 7, !"Dwarf Version", i32 4}
-!8 = !{i32 2, !"Debug Info Version", i32 3}
-!9 = !{i32 1, !"wchar_size", i32 4}
-!10 = distinct !DISubprogram(name: "main", scope: !1, file: !1, line: 16, type: !11, scopeLine: 16, spFlags: DISPFlagDefinition, unit: !0, retainedNodes: !2)
-!11 = !DISubroutineType(types: !12)
-!12 = !{!5}
-!13 = !DILocalVariable(name: "num", scope: !10, file: !1, line: 17, type: !5)
-!14 = !DILocation(line: 0, scope: !10)
-!15 = !{i1 false}
-!16 = !DILocation(line: 18, column: 27, scope: !10)
-!17 = !DILocation(line: 18, column: 30, scope: !10)
-!18 = !DILocation(line: 18, column: 20, scope: !10)
-!19 = !DILocation(line: 18, column: 14, scope: !10)
-!20 = !DILocalVariable(name: "j", scope: !10, file: !1, line: 18, type: !4)
-!21 = !DILocation(line: 19, column: 19, scope: !10)
-!22 = !DILocation(line: 19, column: 16, scope: !10)
-!23 = !DILocation(line: 19, column: 23, scope: !10)
-!24 = !DILocalVariable(name: "nnum", scope: !10, file: !1, line: 19, type: !5)
-!25 = !DILocation(line: 20, column: 10, scope: !10)
-!26 = !DILocation(line: 20, column: 5, scope: !10)
-!27 = !DILocation(line: 38, column: 1, scope: !10)
+!3 = !{!"clang version 10.0.0-4ubuntu1 "}
+!4 = !{i32 7, !"Dwarf Version", i32 4}
+!5 = !{i32 2, !"Debug Info Version", i32 3}
+!6 = !{i32 1, !"wchar_size", i32 4}
+!7 = distinct !DISubprogram(name: "main", scope: !1, file: !1, line: 16, type: !8, scopeLine: 16, spFlags: DISPFlagDefinition, unit: !0, retainedNodes: !2)
+!8 = !DISubroutineType(types: !9)
+!9 = !{!10}
+!10 = !DIBasicType(name: "int", size: 32, encoding: DW_ATE_signed)
+!11 = !{i1 false}
+!12 = !DILocalVariable(name: "a", scope: !7, file: !1, line: 52, type: !13)
+!13 = !DICompositeType(tag: DW_TAG_array_type, baseType: !10, size: 320, elements: !14)
+!14 = !{!15}
+!15 = !DISubrange(count: 10)
+!16 = !DILocation(line: 52, column: 9, scope: !7)
+!17 = !DILocalVariable(name: "num", scope: !7, file: !1, line: 53, type: !10)
+!18 = !DILocation(line: 0, scope: !7)
+!19 = !DILocation(line: 54, column: 14, scope: !7)
+!20 = !DILocation(line: 54, column: 5, scope: !7)
+!21 = !DILocalVariable(name: "__vla_expr0", scope: !7, type: !22, flags: DIFlagArtificial)
+!22 = !DIBasicType(name: "long unsigned int", size: 64, encoding: DW_ATE_unsigned)
+!23 = !DILocalVariable(name: "b", scope: !7, file: !1, line: 54, type: !24)
+!24 = !DICompositeType(tag: DW_TAG_array_type, baseType: !10, elements: !25)
+!25 = !{!26}
+!26 = !DISubrange(count: !21)
+!27 = !DILocation(line: 54, column: 9, scope: !7)
+!28 = !DILocation(line: 55, column: 5, scope: !7)
+!29 = !DILocation(line: 55, column: 10, scope: !7)
+!30 = !DILocation(line: 56, column: 5, scope: !7)
+!31 = !DILocation(line: 56, column: 10, scope: !7)
+!32 = !DILocation(line: 57, column: 19, scope: !7)
+!33 = !DILocalVariable(name: "newname", scope: !7, file: !1, line: 57, type: !10)
+!34 = !DILocation(line: 58, column: 1, scope: !7)
